Unification_solver.v
@@ -1,0 +1,69 @@
+From Licenta Require Import Semantics.
+From Licenta Require Import Syntax.
+
+Require Import String.
+Open Scope string_scope.
+
+Require Import List.
+Import ListNotations.
+
+Inductive solver : unification_problem -> Prop :=
+  | Sbottom : solver Ubottom
+  | Ssolved (u_p : unification_problem) (H : (unification_problem_in_solved_form u_p) = true) : solver u_p
+  | Sdelete (u_p u_p' : unification_problem)(H : ((term_in_unification_problem u_p term_eq) = true)) (H' : (remove_first_appearance_term_unification_problem u_p term_eq) = u_p')(H'' : solver u_p'): solver u_p
+  | Sdecompose (u_p u_p' : unification_problem)(tp : term_pair)(H : ((term_in_unification_problem u_p is_decomposition_term_pair) = true)) (H' : (remove_and_replace_decomposition_unif_problem tp u_p) = u_p')(H'' : solver u_p'): solver u_p
+  | Sorientation (u_p u_p' : unification_problem) (tp : term_pair) (H : ((term_in_unification_problem u_p is_orientation_term_pair) = true)) (H' : (apply_orientation tp u_p) = u_p') (H'' : solver u_p'): solver u_p
+  | Selimination (u_p u_p' : unification_problem) (tp : term_pair) (H : ((term_in_unification_problem u_p is_elimination_term_pair) = true)) (H' : (elimination tp u_p) = u_p') (H'' : solver u_p'): solver u_p
+  | Sconflict (u_p u_p' : unification_problem) (tp : term_pair) (H : ((term_in_unification_problem u_p is_conflict_term_pair) = true)) (H' : (remove_conflict_term_pair tp u_p) = u_p') (H'' : solver u_p'): solver u_p
+  | Soccurs_check (u_p u_p' : unification_problem) (tp : term_pair) (H : ((term_in_unification_problem u_p is_occurs_check_term_pair) = true)) (H' : (occurs_check tp u_p) = u_p') (H'' : solver u_p'): solver u_p.
+
+Theorem test1 : solver unif_probl1.
+  Proof. unfold unif_probl1. apply (Sdelete unif_probl1 (Uset [decomposition_term_pair; orientation_term_pair])).
+  - simpl. reflexivity.
+  - simpl. reflexivity.
+  - apply (Sdecompose (Uset [decomposition_term_pair; orientation_term_pair]) (Uset [orientation_term_pair; Tpair (Tvar x) (Tvar a); Tpair (Tvar y) (Tvar b)]) decomposition_term_pair).
+    -- simpl. reflexivity.
+    -- simpl. reflexivity.
+    -- apply (Sorientation (Uset [orientation_term_pair; Tpair (Tvar x) (Tvar a); Tpair (Tvar y) (Tvar b)]) (Uset [Tpair (Tvar a) t2; Tpair (Tvar x) (Tvar a); Tpair (Tvar y) (Tvar b)]) orientation_term_pair).
+     --- simpl. reflexivity.
+     --- simpl. reflexivity. 
+     --- apply Ssolved. 
+      ---- simpl. reflexivity.
+Qed.
+
+Theorem test2 : solver unif_probl2.
+  Proof. unfold unif_probl2. unfold conflict_term.
+  apply (Sconflict unif_probl2 Ubottom conflict_term).
+  - simpl. reflexivity.
+  - simpl. reflexivity.
+  - apply Sbottom.
+Qed.
+
+Theorem test3 : solver (Uset [occurs_check_term_pair]).
+Proof.
+  apply (Soccurs_check (Uset [occurs_check_term_pair]) Ubottom occurs_check_term_pair).
+  - simpl. reflexivity.
+  - simpl. reflexivity.
+  - apply Sbottom.
+Qed.
+
+Theorem test4 : solver unif_probl4.
+Proof.
+  apply (Sdecompose unif_probl4 unif_probl4' (Tpair (Tfunc f [Tvar x2; Tvar x2]) (Tfunc f [Tvar a; Tvar x1]))).
+  - simpl. reflexivity.
+  - simpl. reflexivity.
+  - apply (Selimination unif_probl4' unif_probl4'' (Tpair (Tvar x2) (Tvar a))).
+    -- simpl. reflexivity.
+    -- simpl. reflexivity.
+    -- apply (Sorientation unif_probl4'' unif_probl4''' (Tpair (Tvar a) (Tvar x1))).
+      --- simpl. reflexivity.
+      --- simpl. reflexivity.
+      --- apply (Selimination unif_probl4''' unif_probl4'''' (Tpair (Tvar x1) (Tvar a))).
+        ---- simpl. reflexivity.
+        ---- simpl. reflexivity.
+        ---- apply (Sorientation unif_probl4'''' unif_probl4''''' (Tpair (Tfunc f [Tfunc g [Tvar a; Tvar a]; Tvar a])(Tvar x3))).
+          ----- simpl. reflexivity.
+          ----- simpl. reflexivity.
+          ----- apply Ssolved. simpl. reflexivity.
+Qed.
+
